Sorted_Terms: moved basic terms

thys/Pattern_Completeness/Pattern_Completeness.thy
@@ -10,16 +10,12 @@ theory Pattern_Completeness
     Pattern_Completeness_Improved_Algorithm
     Show.Shows_Literal
     Certification_Monads.Check_Monad
+    Sorted_Terms.Basic_Terms
 begin
 
+lemmas [iff del] = domIff
 
 text \<open>A pattern completeness decision procedure for a set of lhss\<close>
-
-definition basic_terms :: "('f,'s)ssig \<Rightarrow> ('f,'s)ssig \<Rightarrow> ('v \<rightharpoonup> 's) \<Rightarrow> ('f,'v)term set" (\<open>\<B>'(_,_,_')\<close>) where
-  "\<B>(C,D,V) = { Fun f ts | f ss s ts . f : ss \<rightarrow> s in D \<and> ts :\<^sub>l ss in \<T>(C,V)}" 
-
-abbreviation basic_ground_terms :: "('f,'s)ssig \<Rightarrow> ('f,'s)ssig \<Rightarrow> ('f,unit)term set" (\<open>\<B>'(_,_')\<close>) where
-  "\<B>(C,D) \<equiv> \<B>(C,D,\<lambda>x. None)"
 
 definition matches :: "('f,'v)term \<Rightarrow> ('f,'w)term \<Rightarrow> bool" (infix \<open>matches\<close> 50) where
   "l matches t = (\<exists> \<sigma>. t = l \<cdot> \<sigma>)"
@@ -28,21 +24,20 @@ lemma matches_subst: "l matches t \<Longrightarrow> l matches t\<cdot>\<sigma>"
   by (auto simp: matches_def simp flip: subst_subst_compose) 
 
 definition pat_complete_lhss :: "('f,'s)ssig \<Rightarrow> ('f,'s)ssig \<Rightarrow> ('f,'v)term set \<Rightarrow> bool" where
-  "pat_complete_lhss C D L = (\<forall> t \<in> \<B>(C,D). \<exists>l \<in> L. l matches t)" 
+  "pat_complete_lhss C D L = (\<forall> t \<in> dom \<T>\<^sub>B(C,D). \<exists>l \<in> L. l matches t)" 
 
 lemma pat_complete_lhssD:
-  assumes comp: "pat_complete_lhss C D L" and t: "t \<in> \<B>(C,D,\<emptyset>)"
+  assumes comp: "pat_complete_lhss C D L" and t: "t \<in> dom \<T>\<^sub>B(C,D,\<emptyset>)"
   shows "\<exists>l \<in> L. l matches t" 
 proof -
   note * = map_subst_hastype[OF sorted_map_empty, of C _ _ "\<emptyset>::unit\<rightharpoonup>_" undefined]
-  from t have "t\<cdot>undefined \<in> \<B>(C,D)" (is "?t \<in> _")
-    by (force simp: basic_terms_def * cong: ex_cong)
+  from t have "t\<cdot>undefined \<in> dom \<T>\<^sub>B(C,D)" (is "?t \<in> _")
+    by (auto 0 3 simp: in_dom_iff_ex_type hastype_Basic intro!:*)
   from comp[unfolded pat_complete_lhss_def, rule_format, OF this]
   obtain l where l: "l \<in> L" "l matches ?t" by auto
   from t
   have t2: "?t \<cdot> undefined = t"
-    by (auto simp: basic_terms_def o_def
-        simp: map_subst_subst_Term_empty map_subst_Term_empty_id)
+    by (simp add: in_dom_Basic_empty_subst_subst in_dom_Basic_empty_subst_id)
   from l show "\<exists>l \<in> L. l matches t"
     apply (subst t2[symmetric])
     by (force simp: matches_subst)
@@ -121,7 +116,7 @@ qed
 lemma pats_of_lhss: 
   assumes "isOK(check_signatures C D)" 
   shows  "pats_complete (map_of C) (pat_list ` set (pats_of_lhss D lhss)) = 
-   (\<forall>t\<in>\<B>(map_of C,map_of D). \<exists>l\<in>set lhss. l matches t)" 
+   (\<forall>t \<in> dom \<T>\<^sub>B(map_of C,map_of D). \<exists>l\<in>set lhss. l matches t)" 
 proof -
   define S where "S = sorts_of_ssig_list C"
   note * = check_signatures[OF assms, folded S_def]
@@ -155,7 +150,7 @@ proof -
         cong: all_cong1 ex_cong1 conj_cong imp_cong)
     apply (subst all_comm)
     by (simp add: ac_simps verit_bool_simplify(4) o_def)
-  also have "?L = \<B>(?C,?D,\<emptyset>)" (is "_ = ?R") 
+  also have "?L = dom \<T>\<^sub>B(?C,?D,\<emptyset>)" (is "_ = ?R") 
   proof 
     {
       fix pat and \<sigma>
@@ -176,7 +171,7 @@ proof -
       have ts: "ts :\<^sub>l ss in \<T>(?C)" unfolding list_all2_conv_all_nth ts_def using ssigma by auto
       have pat: "pat \<cdot> \<sigma> = Fun f ts" 
         unfolding pat ts_def by (auto intro: nth_equalityI)
-      from pat f ts have "pat \<cdot> \<sigma> \<in> ?R" unfolding basic_terms_def by auto
+      from pat f ts have "pat \<cdot> \<sigma> \<in> ?R" by (auto simp: in_dom_Basic)
     }
     thus "?L \<subseteq> ?R" by auto
     {
@@ -214,7 +209,7 @@ proof -
       from pat id ssigma
       have "Fun f ts \<in> ?L" by auto
     }
-    thus "?R \<subseteq> ?L" unfolding basic_terms_def by auto
+    thus "?R \<subseteq> ?L" by (auto simp: in_dom_Basic)
   qed
   finally show ?thesis .
 qed
@@ -246,7 +241,7 @@ proof -
     apply (unfold P_def)
     apply (rule pats_of_lhss_vars[OF condD[unfolded P_def S_def]])
     done
-  also have "\<dots> = (\<forall>t\<in>\<B>(?C,?D). \<exists>l\<in>set lhss. l matches t)" unfolding P_def
+  also have "\<dots> = (\<forall>t \<in> dom \<T>\<^sub>B(?C,?D). \<exists>l\<in>set lhss. l matches t)" unfolding P_def
     by (rule pats_of_lhss[OF sig])
   finally show ?thesis unfolding pat_complete_lhss_def .
 qed
@@ -301,7 +296,7 @@ proof -
         by (simp add: distinct_count_atmost_1)
     qed
   qed
-  also have "\<dots> = (\<forall>t\<in>\<B>(?C,?D). \<exists>l\<in>set lhss. l matches t)" unfolding P_def
+  also have "\<dots> = (\<forall>t \<in> dom \<T>\<^sub>B(?C,?D). \<exists>l\<in>set lhss. l matches t)" unfolding P_def
     by (rule pats_of_lhss[OF sig])
   finally show ?thesis unfolding pat_complete_lhss_def .
 qed
@@ -334,7 +329,7 @@ proof -
     apply (unfold P_def)
     apply (rule pats_of_lhss_vars[OF condD[unfolded P_def S_def]])
     done
-  also have "\<dots> = (\<forall>t\<in>\<B>(?C,?D). \<exists>l\<in>set lhss. l matches t)" unfolding P_def
+  also have "\<dots> = (\<forall>t \<in> dom \<T>\<^sub>B(?C,?D). \<exists>l\<in>set lhss. l matches t)" unfolding P_def
     by (rule pats_of_lhss[OF sig])
   finally show ?thesis unfolding pat_complete_lhss_def .
 qed
@@ -343,7 +338,7 @@ text \<open>Definition of strong quasi-reducibility and a corresponding decision
 
 definition strong_quasi_reducible :: "('f,'s)ssig \<Rightarrow> ('f,'s)ssig \<Rightarrow> ('f,'v)term set \<Rightarrow> bool" where
   "strong_quasi_reducible C D L =
-  (\<forall> t \<in> \<B>(C,D). \<exists> ti \<in> set (t # args t). \<exists>l \<in> L. l matches ti)" 
+  (\<forall> t \<in> dom \<T>\<^sub>B(C,D). \<exists> ti \<in> set (t # args t). \<exists>l \<in> L. l matches ti)" 
 
 
 definition term_and_args :: "'f \<Rightarrow> ('f,'v)term list \<Rightarrow> ('f,'v)term list" where
@@ -472,15 +467,15 @@ proof -
       by (auto intro!: nth_equalityI simp: \<sigma>_def)      
     show "\<exists>ti \<in> set (term_and_args f ts). ?match_lhs ti" unfolding id[symmetric] using pat match by auto
   qed
-  also have "\<dots> = (\<forall>t. t \<in> \<B>(?C,?D,\<emptyset>::unit\<rightharpoonup>_) \<longrightarrow> (\<exists> ti \<in> set (t # args t). ?match_lhs ti))"
-    unfolding basic_terms_def term_and_args_def by fastforce
+  also have "\<dots> = (\<forall>t. t \<in> dom \<T>\<^sub>B(?C,?D) \<longrightarrow> (\<exists> ti \<in> set (t # args t). ?match_lhs ti))"
+    unfolding in_dom_Basic term_and_args_def by fastforce
   finally show ?thesis unfolding strong_quasi_reducible_def by blast
 qed
 
 subsection \<open>Connecting Pattern-Completeness, Strong Quasi-Reducibility and Quasi-Reducibility\<close>
 
 definition quasi_reducible :: "('f,'s)ssig \<Rightarrow> ('f,'s)ssig \<Rightarrow> ('f,'v)term set \<Rightarrow> bool" where
-  "quasi_reducible C D L = (\<forall> t \<in> \<B>(C,D). \<exists> tp \<unlhd> t. \<exists>l \<in> L. l matches tp)" 
+  "quasi_reducible C D L = (\<forall>t \<in> dom \<T>\<^sub>B(C,D). \<exists> tp \<unlhd> t. \<exists>l \<in> L. l matches tp)" 
 
 lemma pat_complete_imp_strong_quasi_reducible:
   "pat_complete_lhss C D L \<Longrightarrow> strong_quasi_reducible C D L" 
@@ -505,7 +500,7 @@ proof (standard, rule strong_quasi_reducible_imp_quasi_reducible[OF pat_complete
     unfolding pat_complete_lhss_def
   proof 
     fix t :: "('f,unit)term"
-    assume t: "t \<in> \<B>(C,D,\<emptyset>)"
+    assume t: "t \<in> dom \<T>\<^sub>B(C,D)"
     from q[unfolded quasi_reducible_def, rule_format, OF this]
     obtain tp where tp: "t \<unrhd> tp" and match: "\<exists>l \<in> L. l matches tp" by auto
     show "\<exists>l \<in> L. l matches t" 
@@ -514,13 +509,17 @@ proof (standard, rule strong_quasi_reducible_imp_quasi_reducible[OF pat_complete
       thus ?thesis using match by auto
     next
       case False
-      from t[unfolded basic_terms_def] obtain f ts ss where t: "t = Fun f ts" and ts: "ts :\<^sub>l ss in \<T>(C,\<emptyset>)" by auto
-      from t False tp obtain ti where ti: "ti \<in> set ts" and subt: "ti \<unrhd> tp"
-        by (meson Fun_supteq)
+      from t[unfolded in_dom_Basic]
+      obtain f ts ss where t: "t = Fun f ts" and ts: "ts :\<^sub>l ss in \<T>(C,\<emptyset>)" by auto
+      from t False tp
+      obtain ti where ti: "ti \<in> set ts" and subt: "ti \<unrhd> tp" by (meson Fun_supteq)
       from subt obtain CC where ctxt: "ti = CC \<langle> tp \<rangle>" by auto
-      from ti ts obtain s where "ti : s in \<T>(C)" unfolding list_all2_conv_all_nth set_conv_nth by auto
-      from hastype_context_decompose[OF this[unfolded ctxt]] obtain s where tp: "tp : s in \<T>(C,\<emptyset>)" by blast
-      from match[unfolded matches_def] obtain l \<sigma> where l: "l \<in> L" and match: "tp = l \<cdot> \<sigma>" by auto
+      from ti ts
+      obtain s where "ti : s in \<T>(C)" unfolding list_all2_conv_all_nth set_conv_nth by auto
+      from hastype_context_decompose[OF this[unfolded ctxt]]
+      obtain s where tp: "tp : s in \<T>(C,\<emptyset>)" by blast
+      from match[unfolded matches_def]
+      obtain l \<sigma> where l: "l \<in> L" and match: "tp = l \<cdot> \<sigma>" by auto
       show ?thesis
       proof (cases l)
         case (Var x)
